coq/CallerOkTest.v
@@ -11,7 +11,7 @@ Definition caller_ok_body : com :=
 
 Theorem caller_ok_correct : forall (n : Z),
   n >= 0 ->
-  wp caller_ok_body (fun s => asZ (s "result"%string) >= 0) (updZ empty_state "n"%string n).
+  wp caller_ok_body (wp_normal (fun s => asZ (s "result"%string) >= 0)) (updZ empty_state "n"%string n).
 Proof.
   intros.
   wp_prove.
