coq/StagedFinal.v
@@ -17,12 +17,12 @@ Definition Q2 (a b : Z) : assertion :=
 
 Lemma stage_1_correct : forall (a b : Z),
   (a >= 0)%Z /\ (b >= 0)%Z ->
-  wp s1 (Q1 a b) (upd (upd empty_state "a"%string (VZ a)) "b"%string (VZ b)).
+  wp s1 (wp_normal (Q1 a b)) (upd (upd empty_state "a"%string (VZ a)) "b"%string (VZ b)).
 Proof.
   intros a b [Ha Hb]. wp_reduce. split.
   - unfold lget, upd, updZ; cbn. split; [apply Ha | reflexivity].
   - intro r. intro Hr. split.
-    + unfold Q1; cbn. rewrite Hr. repeat split; auto.
+    + unfold Q1, wp_normal; cbn. rewrite Hr. repeat split; auto.
     + apply (wp_ccall_frame _ "a2"%string nil r).
 Qed.
 
@@ -31,13 +31,13 @@ Lemma stage_2_correct : forall (a b : Z) (s : state),
   (asZ (s "a2"%string) = (a + 1)%Z) -> (isVZ (s "a2"%string) = true) ->
   (asZ (s "a"%string) = a) -> (isVZ (s "a"%string) = true) ->
   (asZ (s "b"%string) = b) -> (isVZ (s "b"%string) = true) ->
-  wp s2 (Q2 a b) s.
+  wp s2 (wp_normal (Q2 a b)) s.
 Proof.
   intros a b s Hb Ha2_eq Ha2_v Ha_eq Ha_v Hb_eq Hb_v.
   wp_reduce. split.
   - unfold asZ, lget. unfold asZ in Hb_eq. rewrite Hb_eq. split; [apply Hb | assumption].
   - intro r. intro Hr. split.
-    + unfold Q2; simpl. unfold lget, asZ in *.
+    + unfold Q2, wp_normal; simpl. unfold lget, asZ in *.
       rewrite Hr, Ha2_eq, Ha_eq, Hb_eq. repeat split; auto.
     + apply (wp_ccall_frame _ "b2"%string nil r).
 Qed.
@@ -45,19 +45,19 @@ Qed.
 Theorem frame_two_calls_staged : forall (a b : Z),
   (a >= 0)%Z /\ (b >= 0)%Z ->
   wp (CSeq (CSeq s1 s2) (CAss "result"%string (APlus (AVar "a2"%string) (AVar "b2"%string))))
-     (fun s => (asZ (s "result"%string) = ((asZ (s "a"%string) + asZ (s "b"%string)) + 2)%Z))
+     (wp_normal (fun s => (asZ (s "result"%string) = ((asZ (s "a"%string) + asZ (s "b"%string)) + 2)%Z)))
      ((upd (upd empty_state "a"%string (VZ a)) "b"%string (VZ b))).
 Proof.
   intros a b [Ha Hb].
-  apply (wp_seq_decompose s1 (CSeq s2 (CAss "result"%string (APlus (AVar "a2"%string) (AVar "b2"%string)))) (Q1 a b) (fun s => (asZ (s "result"%string) = ((asZ (s "a"%string) + asZ (s "b"%string)) + 2)%Z)) _).
+  apply (wp_seq_decompose_normal s1 (CSeq s2 (CAss "result"%string (APlus (AVar "a2"%string) (AVar "b2"%string)))) (Q1 a b) (wp_normal (fun s => (asZ (s "result"%string) = ((asZ (s "a"%string) + asZ (s "b"%string)) + 2)%Z))) _).
   { apply stage_1_correct. split; assumption. }
   { intros s1 Hq. unfold Q1 in Hq.
     destruct Hq as [Ha2_eq [Ha2_v [Ha_eq [Ha_v [Hb_eq Hb_v]]]]].
-    apply (wp_seq_decompose s2 (CAss "result"%string (APlus (AVar "a2"%string) (AVar "b2"%string))) (Q2 a b) (fun s => (asZ (s "result"%string) = ((asZ (s "a"%string) + asZ (s "b"%string)) + 2)%Z)) _).
+    apply (wp_seq_decompose_normal s2 (CAss "result"%string (APlus (AVar "a2"%string) (AVar "b2"%string))) (Q2 a b) (wp_normal (fun s => (asZ (s "result"%string) = ((asZ (s "a"%string) + asZ (s "b"%string)) + 2)%Z))) _).
     { apply (stage_2_correct a b s1 Hb Ha2_eq Ha2_v Ha_eq Ha_v Hb_eq Hb_v). }
     { intros s2 Hq2. unfold Q2 in Hq2.
       destruct Hq2 as [Hb2_eq [Hb2_v [Ha22_eq [Ha22_v [Ha2_eq2 [Ha2_v2 [Hb2_eq2 Hb2_v2]]]]]]].
-      simpl. unfold lget.
+      simpl. unfold wp_normal, lget.
       destruct (s2 "a2"%string) as [za | | | | | | | | | |] eqn:Ea2; simpl;
         try (exfalso; simpl in Ha22_eq; lia).
       destruct (s2 "b2"%string) as [zb | | | | | | | | | |] eqn:Eb2; simpl;
